examples/ghc/lib/CmmType.v
@@ -64,14 +64,11 @@ Instance Default__CmmType : GHC.Err.Default CmmType :=
 
 (* Converted value declarations: *)
 
-(* Translating `instance Outputable__CmmType' failed: OOPS! Cannot find
-   information for class Qualified "Outputable" "Outputable" unsupported *)
+(* Skipping instance Outputable__CmmType of class Outputable *)
 
-(* Translating `instance Outputable__CmmCat' failed: OOPS! Cannot find
-   information for class Qualified "Outputable" "Outputable" unsupported *)
+(* Skipping instance Outputable__CmmCat of class Outputable *)
 
-(* Translating `instance Outputable__Width' failed: OOPS! Cannot find
-   information for class Qualified "Outputable" "Outputable" unsupported *)
+(* Skipping instance Outputable__Width of class Outputable *)
 
 Local Definition Eq___ForeignHint_op_zeze__
    : ForeignHint -> ForeignHint -> bool :=
@@ -103,8 +100,7 @@ Program Instance Eq___CmmCat : GHC.Base.Eq_ CmmCat :=
     k {| GHC.Base.op_zeze____ := Eq___CmmCat_op_zeze__ ;
          GHC.Base.op_zsze____ := Eq___CmmCat_op_zsze__ |}.
 
-(* Translating `instance Show__Width' failed: OOPS! Cannot find information for
-   class Qualified "GHC.Show" "Show" unsupported *)
+(* Skipping instance Show__Width of class Show *)
 
 (* Skipping instance Ord__Width *)
 
