examples/ghc/lib/Unique.v
@@ -54,11 +54,9 @@ Local Definition Uniquable__Unique_getUnique : Unique -> Unique :=
 Program Instance Uniquable__Unique : Uniquable Unique :=
   fun _ k => k {| getUnique__ := Uniquable__Unique_getUnique |}.
 
-(* Translating `instance Outputable__Unique' failed: OOPS! Cannot find
-   information for class Qualified "Outputable" "Outputable" unsupported *)
+(* Skipping instance Outputable__Unique of class Outputable *)
 
-(* Translating `instance Show__Unique' failed: OOPS! Cannot find information for
-   class Qualified "GHC.Show" "Show" unsupported *)
+(* Skipping instance Show__Unique of class Show *)
 
 Definition eqUnique : Unique -> Unique -> bool :=
   fun arg_0__ arg_1__ =>
