examples/ghc/interface-deps.mk
@@ -1,0 +1,5 @@
+$(OUT)/BooleanFormula.v: $(OUT)/SrcLoc.h2ci
+$(OUT)/Name.v: $(OUT)/OccName.h2ci
+$(OUT)/Var.v: $(OUT)/IdInfo.h2ci
+$(OUT)/CoreFVs.v: $(OUT)/CoreType.h2ci
+
